ArkLib/ToVCVio/Lemmas.lean
@@ -6,6 +6,6 @@ section simp_lemmas -- Some extra lemmas that still need to move to vcv
 
 universe u v w
 
-variable {spec : OracleSpec} {α β γ ω : Type u}
+variable {ι} {spec : OracleSpec ι} {α β γ ω : Type u}
 
 end simp_lemmas
